symmetric proofs work well

examples/Sek/View_proof.v
@@ -18,6 +18,14 @@ Require Import View_ml.
 
 
 (* ******************************************************* *)
+(** ** Definitions *)
+
+Definition vswap (v: view_) :=
+	match v with
+	|	Front => Back
+	|	Back => Front
+	end.
+
 Definition vcons A (v: view_) (x: A) (L: list A) :=
 	match v with
 	|	Front => x :: L
@@ -29,3 +37,91 @@ Definition vapp A (v: view_) (L1 L2: list A) :=
 	|	Front => L1 ++ L2
 	|	Back => L2 ++ L1
 	end.
+
+
+(* ******************************************************* *)
+(** ** Lemmas *)
+
+Lemma vswap_vswap : forall v,
+	vswap (vswap v) = v.
+Proof. intros. destruct v; auto. Qed.
+
+
+Lemma length_vcons : forall A v (x: A) (L: list A),
+	length (vcons v x L) = 1 + length L.
+Proof. intros. destruct v; simpl; rew_list~. Qed.
+
+Lemma length_vapp : forall A v (L1 L2: list A),
+	length (vapp v L1 L2) = length L1 + length L2.
+Proof. intros. destruct v; simpl; rew_list~. Qed.
+
+
+Lemma vapp_assoc : forall A v (L1 L2 L3: list A),
+	vapp v (vapp v L1 L2) L3 = vapp v L1 (vapp v L2 L3).
+Proof. intros. destruct v; simpl; rew_list~. Qed.
+
+Lemma vapp_swap : forall A v (L1 L2: list A),
+	vapp (vswap v) L1 L2 = vapp v L2 L1.
+Proof. intros. destruct v; auto. Qed.
+
+
+Lemma vapp_vcons_l : forall A v (x: A) (L1 L2: list A),
+	vapp v (vcons v x L1) L2 = vcons v x (vapp v L1 L2).
+Proof. intros. destruct v; simpl; rew_list~. Qed.
+
+Lemma vcons_vapp : forall A v (x: A) (L1 L2: list A),
+	vcons v x (vapp v L1 L2) = vapp v (vcons v x L1) L2.
+Proof. intros. destruct v; simpl; rew_list~. Qed.
+
+Lemma vapp_vcons_r : forall A v (x: A) (L1 L2: list A),
+	vapp v L1 (vcons v x L2) = vapp v (vcons (vswap v) x L1) L2.
+Proof. intros. destruct v; simpl; rew_list~. Qed.
+
+Lemma vapp_vcons_swap : forall A v (x: A) (L1 L2: list A),
+	vapp v (vcons (vswap v) x L1) L2 = vapp v L1 (vcons v x L2).
+Proof. intros. destruct v; simpl; rew_list~. Qed.
+
+
+Lemma vapp_nil_l : forall A v (L: list A),
+	vapp v nil L = L.
+Proof. intros. destruct v; simpl; rew_list~. Qed.
+
+Lemma vapp_nil_r : forall A v (L: list A),
+	vapp v L nil = L.
+Proof. intros. destruct v; simpl; rew_list~. Qed.
+
+Lemma self_eq_vapp_l_inv : forall A v (L1 L2: list A),
+	L1 = vapp v L1 L2 ->
+	L2 = nil.
+Proof.
+	intros. destruct v; simpl in H.
+	{ applys* self_eq_app_l_inv. }
+	{ applys* self_eq_app_r_inv. }
+Qed.
+
+Lemma self_eq_app_r_inv : forall A v (L1 L2: list A),
+	L2 = vapp v L1 L2 ->
+	L1 = nil.
+Proof. intros. rewrites <- vapp_swap in H. applys* self_eq_vapp_l_inv. Qed.
+
+
+(* ******************************************************* *)
+(** ** Hints *)
+
+Hint Rewrite vswap_vswap : rew_list.
+Hint Rewrite length_vcons length_vapp : rew_list.
+Hint Rewrite vapp_assoc vapp_swap : rew_list.
+Hint Rewrite vcons_vapp vapp_vcons_l vapp_vcons_swap vapp_vcons_r : rew_list.
+Hint Rewrite vapp_nil_l vapp_nil_r self_eq_vapp_l_inv self_eq_app_r_inv : rew_list.
+
+
+(* ******************************************************* *)
+(** ** Specifications *)
+
+Lemma view_swap_spec : forall (v: view_),
+	SPEC (view_swap v)
+		PRE (\$1)
+		POST \[= vswap v].
+Proof. xcf. xpay. xmatch; xvals~. Qed.
+
+Hint Extern 1 (RegisterSpec view_swap) => Provide view_swap_spec.
